CP in removing last remaining failing instances

src/SizeCorr.ml
@@ -34,11 +34,17 @@ let sameTypeCtr c_ctr = function
   | _ -> false
 
 
+let rec fst_leq_proof ctrs =
+  match ctrs with
+  | [] -> forall_nil (gProd hole hole)
+  | c :: ctrs ->
+     forall_cons (gProd hole hole) ltnOSn_pair (fst_leq_proof ctrs)
+
 let isBaseBranch ty_ctr ty = fold_ty' (fun b ty' -> b && not (sameTypeCtr ty_ctr ty')) true ty
 
 let base_ctrs ty_ctr ctrs = List.filter (fun (_, ty) -> isBaseBranch ty_ctr ty) ctrs
 
-let genCorr ty_ctr ctrs iargs inst_name mon_inst_name =
+let genCorr ty_ctr ctrs iargs inst_name s_inst_name c_inst_name mon_inst_name =
 
   (* Common helpers, refactor? *)
   let coqTyCtr = gTyCtr ty_ctr in
@@ -98,6 +104,21 @@ let genCorr ty_ctr ctrs iargs inst_name mon_inst_name =
   let mon_proof size =
     let args = (List.flatten (List.map (fun x -> [x; hole; hole; hole]) coqTyParams)) @ [size] in
     gApp ~explicit:true mon_inst_name args
+  in
+
+  let g_instance =
+    let args = (List.flatten (List.map (fun x -> [x; hole]) coqTyParams)) in
+    gApp ~explicit:true inst_name args
+  in
+
+  let s_instance =
+    let args = (List.flatten (List.map (fun x -> [x; hole]) coqTyParams)) in
+    gApp ~explicit:true s_inst_name args
+  in  
+
+  let c_instance =
+    let args = (List.flatten (List.map (fun x -> [x; hole; hole]) coqTyParams)) in
+    gApp ~explicit:true c_inst_name args
   in
 
   (* Code that generates the generators. Copy-pasted for the third time. XXX factor it out *)
@@ -168,7 +189,7 @@ let genCorr ty_ctr ctrs iargs inst_name mon_inst_name =
          | [(ctr, ty)] -> proof (gVar ihs) hmon ty 0
          | _ :: _ ->
            set_eq_trans
-             (semFreq gen gens hole)
+             (semFreq gen gens (fst_leq_proof ctrs))
              (genCase (gVar ihs) hmon (gPair (hole, hole)) ctrs))
   in
 
@@ -193,9 +214,8 @@ let genCorr ty_ctr ctrs iargs inst_name mon_inst_name =
   let gen_proof =
     gFun ["n"]
       (fun [n] ->
-         gApp ~explicit:true (gInject "nat_set_ind")
-           [full_dt; hole; hole
-           ; base_case; ind_case (mon_proof (gVar n)); (gVar n)])
+         nat_set_ind
+           full_dt g_instance s_instance c_instance base_case (ind_case (mon_proof (gVar n))) (gVar n))
   in
   msg_debug (str "Sized proof");
   debug_coq_expr gen_proof;
